intermediate/Veritas.Intermediate.Simulation.fst
@@ -1,0 +1,71 @@
+module Veritas.Intermediate.Simulation
+
+module Spec = Veritas.Verifier
+module IC = Veritas.Intermediate.Common
+module IS = Veritas.Intermediate.Store
+module IV = Veritas.Intermediate.Verifier
+
+(* Relation between stores *)
+let store_rel (st:IS.vstore) (st':Spec.vstore) : Type = 
+  // no duplicates in st
+  (forall (s:IC.slot_id{IS.contains_record st s}) 
+     (s':IC.slot_id{IS.contains_record st s'}).
+     IS.get_key_at st s <> IS.get_key_at st s') /\
+  // values is st and st' match -- do we need both directions?
+  (forall (s:IC.slot_id{IS.contains_record st s}).
+     let k = IS.get_key_at st s in 
+     let v = IS.get_value_at st s in
+     let a = IS.get_add_method_at st s in
+     Spec.store_contains st' k /\ 
+     v = Spec.stored_value st' k /\
+     a = Spec.add_method_of st' k) /\
+  (forall (k:Veritas.Key.key{Spec.store_contains st' k}). 
+     let v' = Spec.stored_value st' k in
+     let a' = Spec.add_method_of st' k in
+     IS.contains_key st k /\
+     v' = IS.value_of st k /\
+     a' = IS.add_method_of st k)
+
+(* Relation between thread-local states *)
+let vtls_rel (vs:IV.vtls) (vs':Spec.vtls) : Type =
+  // either both runs failed
+  (IV.Failed? vs /\ Spec.Failed? vs') \/
+  // or vs is not a valid map (which relates to any vs')
+  (IV.Valid? vs /\ not (IV.thread_store_is_map vs)) \/
+  // or vs and vs' have related stores
+  (match vs, vs' with
+   | IV.Valid id st clk ha he, Spec.Valid id' st' clk' _ ha' he' ->
+       store_rel st st' /\ 
+       // other fields related by equality -- may not need? 
+       id = id' /\ clk = clk' /\ ha = ha' /\ he = he'   
+   | _ -> False)
+
+(* Relation between a key and slot id *)
+let slot_key_rel (vs:IV.vtls) (s:IC.slot_id) (k:Veritas.Key.key) : Type =
+  IV.Valid? vs /\ 
+  (not (IV.thread_store_is_map vs) \/ 
+    (let st = IV.Valid?.st vs in
+     IS.contains_record st s && IS.get_key_at st s = k))
+
+(* example simulation statement for vput *)
+let lemma_vput_simulates_spec 
+      (vs:IV.vtls) 
+      (vs':Spec.vtls) 
+      (s:IC.slot_id) 
+      (k:Veritas.Key.data_key) 
+      (v:Veritas.Record.data_value) 
+  : Lemma (requires (vtls_rel vs vs' /\ slot_key_rel vs s k
+                     /\ Spec.Valid? vs' ))
+          (ensures (vtls_rel (IV.vput s v vs) (Spec.vput k v vs'))) 
+  = admit()
+
+// some function that maps a log with keys to a log with slot id's
+// (not sure how that works...)
+let convert_log (l:Spec.vlog) : IV.vlog = admit()
+
+(* End goal: For any log the intermediate implementation will verify 
+   iff the the spec implementation does. *)
+module VT = Veritas.Verifier.Thread
+let lemma_verifiable_simulates_spec (tl:VT.thread_id_vlog) 
+  : Lemma (IV.verifiable (VT.thread_id_of tl) (convert_log (VT.vlog_of tl)) = VT.verifiable tl)
+  = admit()
